theories/Events/MapDefaultFacts.v
@@ -45,7 +45,7 @@ Section MapFacts.
   Lemma lookup_add_eq: forall k v s, lookup k (add k v s) = Some v.
   Proof.
     intros.
-    rewrite mapsto_lookup; apply mapsto_add_eq. 
+    rewrite mapsto_lookup; apply mapsto_add_eq.
     Unshelve.
     2: typeclasses eauto.
   Qed.
@@ -101,7 +101,7 @@ Section MapFacts.
   Global Instance eq_map_refl {d} : Reflexive (@eq_map _ _ _ _ d).
   Proof.
     red. intros. unfold eq_map. tauto.
-  Qed.    
+  Qed.
 
   Global Instance eq_map_sym {d} : Symmetric (@eq_map _ _ _ _ d).
   Proof.
@@ -113,7 +113,7 @@ Section MapFacts.
 
   Global Instance eq_map_trans {d} : Transitive (@eq_map _ _ _ _ d).
   Proof.
-    repeat intro. 
+    repeat intro.
     unfold eq_map in *.
     rewrite H. rewrite H0. reflexivity.
   Qed.
@@ -123,7 +123,7 @@ Section MapFacts.
   Context {R1 R2 : Type}.
   Variable RR : R1 -> R2 -> Prop.
 
-  Definition map_default_eq d {E} 
+  Definition map_default_eq d {E}
     : (stateT map (itree E) R1) -> (stateT map (itree E) R2) -> Prop :=
     fun t1 t2 => forall s1 s2, (@eq_map _ _ _ _ d) s1 s2 -> eutt (prod_rel (@eq_map _ _ _ _ d) RR) (t1 s1) (t2 s2).
 
@@ -141,7 +141,7 @@ Section MapFacts.
       rewrite 2 lookup_add_eq; reflexivity.
     - unfold lookup_default in *.
       rewrite 2 lookup_add_neq; auto.
-  Qed.      
+  Qed.
 
   Lemma eq_map_remove:
     forall (d : V) (s1 s2 : map) (k : K), (@eq_map _ _ _ _ d) s1 s2 -> (@eq_map _ _ _ _ d) (remove k s1) (remove k s2).
@@ -154,8 +154,8 @@ Section MapFacts.
     - rewrite 2 lookup_remove_neq; auto.
       apply H.
   Qed.
-  
-  Lemma handle_map_eq : 
+
+  Lemma handle_map_eq :
     forall d E X (s1 s2 : map) (m : mapE K d X),
       (@eq_map _ _ _ _ d) s1 s2 ->
       eutt (prod_rel (@eq_map _ _ _ _ d) eq) (handle_map m s1) ((handle_map m s2) : itree E (map * X)).
@@ -175,8 +175,8 @@ Section MapFacts.
     apply handle_map_eq.
     assumption.
   Qed.
-    
-  
+
+
   (* This lemma states that the operations provided by [handle_map] respect
      the equivalence on the underlying map interface *)
   Lemma interp_map_id d {E X} (t : itree (mapE K d +' E) X) :
@@ -202,7 +202,7 @@ Section MapFacts.
         gstep; constructor.
         gbase. apply CH. assumption.
   Qed.
- 
+
   Global Instance interp_map_proper {R E d} {RR : R -> R -> Prop} :
     Proper ((eutt RR) ==> (@map_default_eq _ _ RR d E)) (@interp_map _ _ _ _ E d R).
   Proof.
@@ -212,7 +212,7 @@ Section MapFacts.
     einit.
     ecofix CH.
     intros.
-    rewrite! unfold_interp_state. 
+    rewrite! unfold_interp_state.
     punfold H0. red in H0.
     revert s1 s2 H1.
     induction H0; intros; subst; simpl; pclearbot.
@@ -225,7 +225,7 @@ Section MapFacts.
         destruct e. apply handle_map_eq. assumption.
         unfold pure_state.
         pstep. econstructor. intros. constructor. pfold. econstructor. constructor; auto.
-      } 
+      }
       intros.
       inversion H. subst.
       estep; constructor. ebase.
@@ -234,5 +234,5 @@ Section MapFacts.
     - rewrite tau_eutt, unfold_interp_state.
       eauto.
   Qed.
-    
+
 End MapFacts.
